1. Simplify: \(\displaystyle \frac{2x^{2}-8}{2x}\).

2. Solve for \(x\): \(3(x-2)=2x+5\).

3. Solve the quadratic: \(x^{2}-5x+6=0\).

4. Factor completely: \(x^{3}-6x^{2}+11x-6\).

5. Simplify and state excluded values: \(\displaystyle \frac{x^{2}-9}{x^{2}-x-6}\).

6. Find the domain of \(f(x)=\displaystyle \frac{\sqrt{x-2}}{x-4}\).

7. Given \(f(x)=2x+3\) and \(g(x)=x^{2}\), compute \((f\circ g)(-2)\) and \((g\circ f)(1)\).

8. Find the inverse function: \(f(x)=\dfrac{3x-2}{5}\). (Give \(f^{-1}(x)\).)

9. Solve for \(x\): \(2^{\,x+1}=16\).

10. Solve for \(x\): \(\log\_{3}\!\bigl(x^{2}-1\bigr)=2\). (State valid solutions.)

11. Evaluate the trigonometric value: \(\sin\!\bigl(\tfrac{5\pi}{6}\bigr)\).

12. Simplify the identity: \(\sin^{2}x+\cos^{2}x\).

13. Solve on \([0,2\pi)\): \(\sin x=\tfrac{1}{2}\).

14. Let \(f(x)=\begin{cases}x^{2},&x\le 1,\\[4pt]2x+1,&x>1.\end{cases}\)  
    (a) Find \(f(1)\).  
    (b) Compute \(\displaystyle\lim*{x\to1^{-}} f(x)\) and \(\displaystyle\lim*{x\to1^{+}} f(x)\).  
    (c) Is \(f\) continuous at \(x=1\)?

15. Solve the absolute inequality: \(|2x-3|<5\).

16. Solve the rational inequality: \(\dfrac{x-1}{x+2}\ge 0\). (Give interval answer.)

17. Compute and simplify the difference quotient for \(f(x)=x^{2}+2x\):  
    \(\displaystyle \frac{f(x+h)-f(x)}{h}\).

18. Find the average rate of change of \(f(x)=\dfrac{1}{x}\) between \(x=1\) and \(x=3\).

19. For \(f(x)=(x-2)(x+1)\):  
    (a) Identify the \(x\)-intercepts.  
    (b) Find the \(y\)-intercept.  
    (c) Describe end behavior.

20. Determine whether \(f(x)=x^{3}-x\) is even, odd, or neither.

---

## 1. Simplify: \(\displaystyle \frac{2x^{2}-8}{2x}\).

**Answer: ** \(\displaystyle \frac{(x-2)(x+2)}{x}\)

## 2. Solve for \(x\): \( 3(x - 2) = 2x + 5 \)

### Step 1: Distribute the 3 on the left-hand side:

\[
3(x - 2) = 3x - 6
\]
So the equation becomes:
\[
3x - 6 = 2x + 5
\]

### Step 2: Move all terms involving \(x\) to one side. Subtract \(2x\) from both sides:

\[
3x - 2x - 6 = 5
\]
Simplifying:
\[
x - 6 = 5
\]

### Step 3: Isolate \(x\) by adding 6 to both sides:

\[
x = 5 + 6
\]
\[
x = 11
\]

The solution is \( x = 11 \).

## 3. Solve the quadratic: \(x^{2}-5x+6=0\).

### Solution

Factor the quadratic:
\[
x^{2}-5x+6=(x-2)(x-3)=0.
\]
Thus the solutions are
\[
x=2\quad\text{or}\quad x=3.
\]

## 4. Factor completely: \(x^{3}-6x^{2}+11x-6\).

### Solution

Try integer roots (1,2,3). Evaluate at \(x=1\): \(1-6+11-6=0\), so \(x-1\) is a factor. Perform synthetic or polynomial division:
\[
x^{3}-6x^{2}+11x-6=(x-1)(x^{2}-5x+6)=(x-1)(x-2)(x-3).
\]

## 5. Simplify and state excluded values: \(\displaystyle \frac{x^{2}-9}{x^{2}-x-6}\).

### Solution

Factor numerator and denominator:
\[
\frac{x^{2}-9}{x^{2}-x-6}=\frac{(x-3)(x+3)}{(x-3)(x+2)}.
\]
For \(x\neq 3\) we cancel \(x-3\) to get
\[
\frac{x+3}{x+2},
\]
but we must exclude values that make the original denominator zero: \(x=3\) and \(x=-2\).

## 6. Find the domain of \(f(x)=\displaystyle \frac{\sqrt{x-2}}{x-4}\).

### Solution

The square root requires \(x-2\ge0\Rightarrow x\ge2\). The denominator cannot be zero, so \(x\neq4\). Therefore the domain is
\[
[2,4)\cup(4,\infty).
\]

## 7. Given \(f(x)=2x+3\) and \(g(x)=x^{2}\), compute \((f\circ g)(-2)\) and \((g\circ f)(1)\).

### Solution

\((f\circ g)(-2)=f(g(-2))=f(4)=2\cdot4+3=11.\)

\((g\circ f)(1)=g(f(1))=g(2\cdot1+3)=g(5)=5^{2}=25.\)

## 8. Find the inverse function: \(f(x)=\dfrac{3x-2}{5}\). (Give \(f^{-1}(x)\).)

### Solution

Set \(y=\dfrac{3x-2}{5}\), solve for \(x\):
\[
5y=3x-2\Rightarrow 3x=5y+2\Rightarrow x=\frac{5y+2}{3}.
\]
Swap \(x\) and \(y\) to write the inverse:
\[
f^{-1}(x)=\frac{5x+2}{3}.
\]

## 9. Solve for \(x\): \(2^{\,x+1}=16\).

### Solution

Write 16 as a power of 2: \(16=2^{4}\). Then
\[
2^{x+1}=2^{4}\Rightarrow x+1=4\Rightarrow x=3.
\]

## 10. Solve for \(x\): \(\log\_{3}\!\bigl(x^{2}-1\bigr)=2\). (State valid solutions.)

### Solution

Convert to exponential form:
\[
x^{2}-1=3^{2}=9\Rightarrow x^{2}=10\Rightarrow x=\pm\sqrt{10}.
\]
Check domain: we need \(x^{2}-1>0\) which holds for \(x=\pm\sqrt{10}\). Thus both are valid.

## 11. Evaluate the trigonometric value: \(\sin\!\bigl(\tfrac{5\pi}{6}\bigr)\).

### Solution

\(\tfrac{5\pi}{6}=\pi-\tfrac{\pi}{6}\). Using the sine of a supplementary angle:
\[
\sin\left(\pi-\tfrac{\pi}{6}\right)=\sin\tfrac{\pi}{6}=\tfrac{1}{2}.
\]

## 12. Simplify the identity: \(\sin^{2}x+\cos^{2}x\).

### Solution

This is the Pythagorean identity:
\[
\sin^{2}x+\cos^{2}x=1.
\]

## 13. Solve on \([0,2\pi)\): \(\sin x=\tfrac{1}{2}\).

### Solution

On \([0,2\pi)\) the solutions are the reference angle \(\pi/6\) in QI and its supplement in QII, so
\[
x=\frac{\pi}{6},\ \frac{5\pi}{6}.
\]

## 14. Let \(f(x)=\begin{cases}x^{2},&x\le 1,\\[4pt]2x+1,&x>1.\end{cases}\)

\(\text{(a) Find }f(1).\)

### Solution (a)

Since \(1\le1\) we use the first branch: \(f(1)=1^{2}=1.\)

\(\text{(b) Compute }\displaystyle\lim*{x\to1^{-}} f(x)\text{ and }\displaystyle\lim*{x\to1^{+}} f(x).\)

### Solution (b)

Left-hand limit: \(\lim*{x\to1^{-}} f(x)=\lim*{x\to1} x^{2}=1.\)
Right-hand limit: \(\lim*{x\to1^{+}} f(x)=\lim*{x\to1} (2x+1)=3.\)

\(\text{(c) Is }f\text{ continuous at }x=1?\)

### Solution (c)

Because the left and right limits are not equal (1 vs 3), \(\lim\_{x\to1} f(x)\) does not exist, so \(f\) is \emph{not} continuous at \(x=1\).

## 15. Solve the absolute inequality: \(|2x-3|<5\).

### Solution

Solve the compound inequality:
\[
-5<2x-3<5\Rightarrow -2<2x<8\Rightarrow -1<x<4.
\]
So the solution set is \((-1,4)\).

## 16. Solve the rational inequality: \(\dfrac{x-1}{x+2}\ge 0\). (Give interval answer.)

### Solution

Critical points: numerator zero at \(x=1\) (gives value 0), denominator zero at \(x=-2\) (excluded). Use sign chart or test intervals:
\[
(-\infty,-2):\;\text{positive},\quad (-2,1):\;\text{negative},\quad (1,\infty):\;\text{positive}.
\]
Include \(x=1\) since the fraction equals 0 there. Exclude \(x=-2\). Thus the solution is
\[
(-\infty,-2)\cup[1,\infty).
\]

## 17. Compute and simplify the difference quotient for \(f(x)=x^{2}+2x\):

\[\displaystyle \frac{f(x+h)-f(x)}{h}.\]

### Solution

Compute \(f(x+h)=(x+h)^{2}+2(x+h)=x^{2}+2xh+h^{2}+2x+2h.\) Then
\[
\frac{f(x+h)-f(x)}{h}=\frac{2xh+h^{2}+2h}{h}=2x+h+2.
\]
So the simplified difference quotient is \(2x+h+2\).

## 18. Find the average rate of change of \(f(x)=\dfrac{1}{x}\) between \(x=1\) and \(x=3\).

### Solution

Average rate of change = \(\dfrac{f(3)-f(1)}{3-1}=\dfrac{1/3-1}{2}=\dfrac{-2/3}{2}=-\dfrac{1}{3}.\)

## 19. For \(f(x)=(x-2)(x+1)\):

### Solution

\(f(x)=0\) when \(x=2\) or \(x=-1\), so the \(x\)-intercepts are \((2,0)\) and \((-1,0)\).

The \(y\)-intercept is \(f(0)=(0-2)(0+1)=-2\), so \((0,-2)\).

End behavior: since the leading term is \(x^{2}\) (positive), \(f(x)\to+\infty\) as \(x\to\pm\infty\) (both ends up).

## 20. Determine whether \(f(x)=x^{3}-x\) is even, odd, or neither.

### Solution

Compute \(f(-x)=(-x)^{3}-(-x)=-x^{3}+x=-(x^{3}-x)=-f(x).\) Therefore \(f\) is an \emph{odd} function.

## 4. Factor completely: \(x^{3}-6x^{2}+11x-6\).

## 5. Simplify and state excluded values: \(\displaystyle \frac{x^{2}-9}{x^{2}-x-6}\).

## 6. Find the domain of \(f(x)=\displaystyle \frac{\sqrt{x-2}}{x-4}\).

## 7. Given \(f(x)=2x+3\) and \(g(x)=x^{2}\), compute \((f\circ g)(-2)\) and \((g\circ f)(1)\).

## 8. Find the inverse function: \(f(x)=\dfrac{3x-2}{5}\). (Give \(f^{-1}(x)\).)

## 9. Solve for \(x\): \(2^{\,x+1}=16\).

## 10. Solve for \(x\): \(\log\_{3}\!\bigl(x^{2}-1\bigr)=2\). (State valid solutions.)

## 11. Evaluate the trigonometric value: \(\sin\!\bigl(\tfrac{5\pi}{6}\bigr)\).

## 12. Simplify the identity: \(\sin^{2}x+\cos^{2}x\).

## 13. Solve on \([0,2\pi)\): \(\sin x=\tfrac{1}{2}\).

## 14. Let \(f(x)=\begin{cases}x^{2},&x\le 1,\\[4pt]2x+1,&x>1.\end{cases}\)

    (a) Find \(f(1)\).
    (b) Compute \(\displaystyle\lim*{x\to1^{-}} f(x)\) and \(\displaystyle\lim*{x\to1^{+}} f(x)\).
    (c) Is \(f\) continuous at \(x=1\)?

## 15. Solve the absolute inequality: \(|2x-3|<5\).

## 16. Solve the rational inequality: \(\dfrac{x-1}{x+2}\ge 0\). (Give interval answer.)

## 17. Compute and simplify the difference quotient for \(f(x)=x^{2}+2x\):

    \(\displaystyle \frac{f(x+h)-f(x)}{h}\).

## 18. Find the average rate of change of \(f(x)=\dfrac{1}{x}\) between \(x=1\) and \(x=3\).

## 19. For \(f(x)=(x-2)(x+1)\):

    (a) Identify the \(x\)-intercepts.
    (b) Find the \(y\)-intercept.
    (c) Describe end behavior.

## 20. Determine whether \(f(x)=x^{3}-x\) is even, odd, or neither.
